lib/falcon/nth_root.dfy
@@ -17,7 +17,9 @@ module nth_root {
 	ghost const OMEGA: elem;
 	ghost const OMEGA_INV: elem;
 	ghost const R: elem;
+	ghost const R2: elem;
 	ghost const R_INV: elem;
+	ghost const N_INV: elem;
 
 	function method {:axiom} montmul(a: elem, b: elem): (c: elem)
 		ensures c == (a * b * R_INV) % Q
@@ -33,6 +35,9 @@ module nth_root {
 		ensures (OMEGA * OMEGA_INV) % Q == 1
 
 		ensures (R_INV * R) % Q == 1
+		ensures IsModEquivalent(R2, R * R, Q); 
+
+		ensures (N_INV * N.full) % Q == 1;
 
 	lemma primitive_root_non_zero_lemma(i: nat)
 		requires i < N.full * 2;
@@ -422,4 +427,12 @@ module nth_root {
 		var _ := twiddle_factors_index_bound_lemma(t, j);
 		rev_omega_inv_powers_mont_table_axiom(t, d, j);
 	}
+
+	function method {:axiom} inverse_ntt_scaling_table(): (t: seq<elem>)
+		ensures |t| == N.full;
+
+	lemma {:axiom} inverse_ntt_scaling_table_axiom(i: nat)
+		requires i < N.full;
+		ensures inverse_ntt_scaling_table()[i] == mqmul(mqmul(mqpow(PSI_INV, i), N_INV), R);
+
 }
